quite a lot of refactoring + decoding of numerics: has all instructions, but some are bogus (eg, const_f cos we don't have ieee754 stuff)

compiler/wasm/wasm_enc_decScript.sml
@@ -1,54 +1,124 @@
 (*
-  Encoding and decoding
+  Encoding and decoding between Cake-Wasm AST & Wasm binary format
 *)
+(* Currently only handling positive numbers *)
 open preamble;
 open wasmLangTheory wordsTheory wordsLib;
 
+(*  TODOs
+    - unsigned LEB
+    - finish up numeric instructions
+    - more of the AST
+    - parser for the decoder
+    - right now LEB decoding takes a detour through HOL nums;
+      would a better route be straight to words?
+ *)
+
 val _ = new_theory "wasm_enc_dec";
 
-(* --- basic LEB128 functions --- *)
+(* --- basic leb functions --- *)
 
 Type byte[local]       = “:word8”
 Type byteStream[local] = “:word8 list”
 
+(*******************)
+(*                 *)
+(*     LEB128      *)
+(*                 *)
+(*******************)
+
+  (***************)
+  (*   Helpers   *)
+  (***************)
+  (* for maintaining an leb abstraction *)
 Overload        n128[local] = “(128:num)”
 Overload     under7b[local] = “λ n. (n <   n128)”         (* : num -> bool    *)
 Overload      last7b[local] = “λ n. (n MOD n128)”         (* : num -> num     *)
 Overload sans_last7b[local] = “λ n. (n DIV n128)”         (* : num -> num     *)
 Overload     not_MSB[local] = “word_msb”                  (* : α word -> bool *)
 Overload      mk_lsB[local] = “λ n.128w + n2w (last7b n)” (* : num -> byte    *)
+Overload  leb_append[local] = “λ pre post. pre * n128 + last7b post”
 (*  under7b := is a num representable in 7 bits
      last7b := the last 7 bits of the binary rep of a num
-sans_last7b := binary rep of a num with last 7 bits truncated
-    not_MSB := not the most sig Byte of a LEB128 encoded int
-     mk_lsB := LEB128 encode 7 bits into a less significant (than the most) Byte *)
+sans_last7b := num with last 7 bits of its binary rep truncated
+    not_MSB := not the most sig Byte of a leb encoded int
+     mk_lsB := leb encode 7 bits into a less significant (than the most) Byte
+ leb_append := "append" a less-sig byte (post) to the end
+                of under-construction number (pre) *)
 
-Definition read_num_def:
-  read_num [] = NONE ∧
-  read_num (b::rest) =
-    if word_msb (b:word8) then
-      case read_num rest of
+(* Magnus orig code *)
+  (* Definition read_num_def:
+    read_num [] = NONE ∧
+    read_num (b::rest) =
+      if word_msb (b:word8) then
+        case read_num rest of
+        | NONE => NONE
+        | SOME (n,left_over) => SOME (w2n b MOD 128 + 128 * n, left_over)
+      else SOME (w2n b, rest)
+  End
+
+  Definition encode_num_def:
+    encode_num n =
+      if n < 128 then [(n2w n):word8] else
+        n2w (n MOD 128) + 128w :: encode_num (n DIV 128)
+  End
+
+  Theorem read_num_encode_num:
+    ∀n rest. read_num (encode_num n ++ rest) = SOME (n,rest)
+  Proof
+    ho_match_mp_tac encode_num_ind \\ rw []
+    \\ simp [Once encode_num_def] \\ rw []
+    >-
+    (simp [Once read_num_def]
+      \\ ‘n DIV 128 = 0’ by gvs [DIV_EQ_X]
+      \\ simp [word_msb_n2w,bitTheory.BIT_DEF])
+    \\ simp [Once read_num_def,word_add_n2w]
+    \\ simp [word_msb_n2w,bitTheory.BIT_DEF]
+    \\ ‘0 < 128:num’ by fs []
+    \\ drule ADD_DIV_ADD_DIV
+    \\ disch_then $ qspecl_then [‘1’] assume_tac
+    \\ gvs []
+    \\ ‘(n MOD 128 + 128) < 256’ by
+    (‘n MOD 128 < 128’ by simp [MOD_LESS]
+      \\ decide_tac)
+    \\ simp [LESS_MOD]
+    \\ ‘0 < 128:num’ by fs []
+    \\ drule DIVISION
+    \\ disch_then (fn th => CONV_TAC (RAND_CONV $ ONCE_REWRITE_CONV [th]))
+    \\ gvs []
+  QED *)
+(* End Magnus orig code *)
+
+(* uleb decode a HOL num from a byte stream *)
+Definition decode_num_def:
+  decode_num ([]:byteStream) : (num # byteStream) option = NONE ∧
+  decode_num (b::rest) =
+    let bn = w2n b in
+    if not_MSB b then
+      case decode_num rest of
+      | SOME (n, left_over) => SOME (leb_append n bn, left_over)
       | NONE => NONE
-      | SOME (n,left_over) => SOME (w2n b MOD 128 + 128 * n, left_over)
-    else SOME (w2n b, rest)
+    else SOME (bn, rest)
 End
 
-Definition num_to_leb128_def:
-  num_to_leb128 n =
-    if n < 128 then [(n2w n):word8] else
-      n2w (n MOD 128) + 128w :: num_to_leb128 (n DIV 128)
+(* uleb encode a (+ve) HOL num to bytes *)
+Definition encode_num_def:
+  encode_num (n:num) : byteStream =
+    if n < 128 then [n2w n]
+    else n2w (n MOD 128) + 128w :: encode_num (n DIV 128)
 End
 
-Theorem read_num_num_to_leb128:
-  ∀n rest. read_num (num_to_leb128 n ++ rest) = SOME (n,rest)
+(* TODO : Documentation *)
+Theorem dec_enc_num_id:
+  ∀n rest. decode_num (encode_num n ++ rest) = SOME (n,rest)
 Proof
-  ho_match_mp_tac num_to_leb128_ind \\ rw []
-  \\ simp [Once num_to_leb128_def] \\ rw []
+  ho_match_mp_tac encode_num_ind \\ rw []
+  \\ simp [Once encode_num_def] \\ rw []
   >-
-   (simp [Once read_num_def]
+   (simp [Once decode_num_def]
     \\ ‘n DIV 128 = 0’ by gvs [DIV_EQ_X]
     \\ simp [word_msb_n2w,bitTheory.BIT_DEF])
-  \\ simp [Once read_num_def,word_add_n2w]
+  \\ simp [Once decode_num_def,word_add_n2w]
   \\ simp [word_msb_n2w,bitTheory.BIT_DEF]
   \\ ‘0 < 128:num’ by fs []
   \\ drule ADD_DIV_ADD_DIV
@@ -64,77 +134,84 @@ Proof
   \\ gvs []
 QED
 
-
-Definition read_word_def:
-  read_word input = case read_num input of
+(* read (unencoded) word out of uleb stream; "polymorphic" *)
+Definition read_u_word_def:
+  read_u_word (input:byteStream) = case decode_num input of
   | SOME (n,rest) => if n < dimword(:α) then SOME ((n2w n):α word, rest) else NONE
   | NONE => NONE
 End
 
-Overload read_byte    = “read_word : byteStream -> (byte    # byteStream) option”
-Overload read_4bytes  = “read_word : byteStream -> (word32  # byteStream) option”
-Overload read_8bytes  = “read_word : byteStream -> (word64  # byteStream) option”
-Overload read_16bytes = “read_word : byteStream -> (word128 # byteStream) option”
-
-Definition write_word_def:
-  write_word (x:(α word)) acc = (num_to_leb128 (w2n x)) ++ acc
+Definition write_u_word_def:
+  write_u_word (x:(α word)) (acc:byteStream) : byteStream = (encode_num (w2n x)) ++ acc
 End
 
-Overload write_byte    = “write_word : byte    -> byteStream -> byteStream”
-Overload write_4bytes  = “write_word : word32  -> byteStream -> byteStream”
-Overload write_8bytes  = “write_word : word64  -> byteStream -> byteStream”
-Overload write_16bytes = “write_word : word128 -> byteStream -> byteStream”
+Overload read_u_B   = “read_u_word : byteStream -> (byte    # byteStream) option”
+Overload read_u_4B  = “read_u_word : byteStream -> (word32  # byteStream) option”
+Overload read_u_8B  = “read_u_word : byteStream -> (word64  # byteStream) option”
+Overload read_u_16B = “read_u_word : byteStream -> (word128 # byteStream) option”
 
-Definition read_w8_def:
-  read_w8 input =
-    case read_num input of
-    | NONE => NONE
-    | SOME (n,rest) => if n < 256 then SOME ((n2w n):word8, rest) else NONE
-End
+(* TODO: implement signed leb *)
+Overload read_s_B   = “read_u_B  ”
+Overload read_s_4B  = “read_u_4B ”
+Overload read_s_8B  = “read_u_8B ”
+Overload read_s_16B = “read_u_16B”
 
-Definition read_w32_def:
-  read_w32 input =
-    case read_num input of
-    | NONE => NONE
-    | SOME (n,rest) => if n < 2**32 then SOME ((n2w n):word32, rest) else NONE
-End
+(* TODO: floats *)
+Overload read_f_B   = “read_u_B  ”
+Overload read_f_4B  = “read_u_4B ”
+Overload read_f_8B  = “read_u_8B ”
+Overload read_f_16B = “read_u_16B”
 
-Definition write_w8_def:
-  write_w8 (x:word8) acc = (num_to_leb128 (w2n x)) ++ acc
-End
+Overload write_u_B   = “write_u_word : byte    -> byteStream -> byteStream”
+Overload write_u_4B  = “write_u_word : word32  -> byteStream -> byteStream”
+Overload write_u_8B  = “write_u_word : word64  -> byteStream -> byteStream”
+Overload write_u_16B = “write_u_word : word128 -> byteStream -> byteStream”
 
-Definition write_w32_def:
-  write_w32 (x:word32) acc = (num_to_leb128 (w2n x)) ++ acc
-End
-
-Theorem read_w8_thm[simp]:
-  read_w8 (write_w8 x rest) = SOME (x,rest)
+Theorem read_write_u_B[simp]:
+  read_u_B (write_u_B x rest) = SOME (x, rest)
 Proof
-  simp [write_w8_def,read_w8_def,read_num_num_to_leb128]
+  simp [read_u_word_def,dec_enc_num_id,write_u_word_def]
   \\ irule LESS_LESS_EQ_TRANS
   \\ irule_at Any w2n_lt \\ simp []
 QED
 
-Theorem read_w32_thm[simp]:
-  read_w32 (write_w32 x rest) = SOME (x,rest)
+Theorem read_write_u_4B[simp]:
+  read_u_4B (write_u_4B x rest) = SOME (x, rest)
 Proof
-  simp [write_w32_def,read_w32_def,read_num_num_to_leb128]
+  simp [read_u_word_def,dec_enc_num_id,write_u_word_def]
   \\ irule LESS_LESS_EQ_TRANS
   \\ irule_at Any w2n_lt \\ simp []
 QED
+
+Theorem read_write_u_8B[simp]:
+  read_u_8B (write_u_8B x rest) = SOME (x, rest)
+Proof
+  simp [read_u_word_def,dec_enc_num_id,write_u_word_def]
+  \\ irule LESS_LESS_EQ_TRANS
+  \\ irule_at Any w2n_lt \\ simp []
+QED
+
+Theorem read_write_u_16B[simp]:
+  read_u_16B (write_u_16B x rest) = SOME (x, rest)
+Proof
+  simp [read_u_word_def,dec_enc_num_id,write_u_word_def]
+  \\ irule LESS_LESS_EQ_TRANS
+  \\ irule_at Any w2n_lt \\ simp []
+QED
+
 
 (* --- example --- *)
 
 Definition encode_def:
   encode (b1,b2,b3) =
-    write_w8 b1 (write_w8 b2 (write_w8 b3 []))
+    write_u_B b1 (write_u_B b2 (write_u_B b3 []))
 End
 
 Definition decode_def:
   decode input =
-    case read_w8 input of NONE => NONE | SOME (b1,input) =>
-    case read_w8 input of NONE => NONE | SOME (b2,input) =>
-    case read_w8 input of NONE => NONE | SOME (b3,input) =>
+    case read_u_B input of NONE => NONE | SOME (b1,input) =>
+    case read_u_B input of NONE => NONE | SOME (b2,input) =>
+    case read_u_B input of NONE => NONE | SOME (b3,input) =>
       if input = [] then SOME (b1,b2,b3) else NONE
 End
 
@@ -144,5 +221,255 @@ Proof
   PairCases
   \\ simp [encode_def,decode_def]
 QED
+
+(* --- example --- *)
+
+
+
+(***********************************************)
+(*                                             *)
+(*     Wasm Binary Format ⇔ WasmCake AST      *)
+(*                                             *)
+(***********************************************)
+
+  (***************)
+  (*   Helpers   *)
+  (***************)
+
+Overload selWidth = “λbool. if bool then W64      else W32”
+Overload selSign  = “λbool. if bool then Unsigned else Signed”
+
+
+
+  (****************)
+  (*   Numtypes   *)
+  (****************)
+
+Definition decode_numtype_def:
+  decode_numtype (b:byte) : numtype option =
+  (* QQ Why not case? MM: this is better. Explanation elided for now *)
+  if b = 0x7Fw then SOME (NT Int   W32) else
+  if b = 0x7Ew then SOME (NT Int   W64) else
+  if b = 0x7Dw then SOME (NT Float W32) else
+  if b = 0x7Cw then SOME (NT Float W64) else NONE
+End
+
+Definition encode_numtype_def:
+  encode_numtype (t:numtype) : byte = case t of
+  | (NT Int   W32) => 0x7Fw
+  | (NT Int   W64) => 0x7Ew
+  | (NT Float W32) => 0x7Dw
+  | (NT Float W64) => 0x7Cw
+End
+
+Theorem dec_enc_numtype[simp]:
+  ∀ t. decode_numtype (encode_numtype t) = SOME t
+Proof
+  Cases >> Cases_on `b` >> Cases_on `w` >>
+  simp[decode_numtype_def, encode_numtype_def]
+QED
+
+(* TODO *)
+(* Theorem enc_dec_numtype:
+  ∀ b t. decode_numtype b = Some t ⇒ (encode_numtype t) = b
+Proof
+  Cases_on `t` >> Cases_on `b` >> Cases_on `w` >>
+  Cases_on `n`
+
+  simp[decode_numtype_def, encode_numtype_def]
+QED *)
+
+  (****************************)
+  (*   Numeric Instructions   *)
+  (****************************)
+
+(* decode a numeric instruction from a stream of bytes. *)
+(*  NB: numeric instructions are variable length as some take numbers as part of their encoding
+    eg constant functions *)
+Definition decode_numI_def:
+  decode_numI ([]:byteStream) : (num_instr option # byteStream) = (NONE, []) ∧
+  decode_numI (b::bs) = let default = (NONE,b::bs) in
+
+  if b = 0x45w then (SOME   (N_test       (Eqz W32)                    ), bs) else
+  if b = 0x46w then (SOME   (N_compare    (Eq Int W32)                 ), bs) else
+  if b = 0x47w then (SOME   (N_compare    (Ne Int W32)                 ), bs) else
+  if b = 0x48w then (SOME   (N_compare    (Lt_   Signed W32)           ), bs) else
+  if b = 0x49w then (SOME   (N_compare    (Lt_ Unsigned W32)           ), bs) else
+  if b = 0x4Aw then (SOME   (N_compare    (Gt_   Signed W32)           ), bs) else
+  if b = 0x4Bw then (SOME   (N_compare    (Gt_ Unsigned W32)           ), bs) else
+  if b = 0x4Cw then (SOME   (N_compare    (Le_   Signed W32)           ), bs) else
+  if b = 0x4Dw then (SOME   (N_compare    (Le_ Unsigned W32)           ), bs) else
+  if b = 0x4Ew then (SOME   (N_compare    (Ge_   Signed W32)           ), bs) else
+  if b = 0x4Fw then (SOME   (N_compare    (Ge_ Unsigned W32)           ), bs) else
+  if b = 0x50w then (SOME   (N_test       (Eqz W64)                    ), bs) else
+  if b = 0x51w then (SOME   (N_compare    (Eq Int W64)                 ), bs) else
+  if b = 0x52w then (SOME   (N_compare    (Ne Int W64)                 ), bs) else
+  if b = 0x53w then (SOME   (N_compare    (Lt_   Signed W64)           ), bs) else
+  if b = 0x54w then (SOME   (N_compare    (Lt_ Unsigned W64)           ), bs) else
+  if b = 0x55w then (SOME   (N_compare    (Gt_   Signed W64)           ), bs) else
+  if b = 0x56w then (SOME   (N_compare    (Gt_ Unsigned W64)           ), bs) else
+  if b = 0x57w then (SOME   (N_compare    (Le_   Signed W64)           ), bs) else
+  if b = 0x58w then (SOME   (N_compare    (Le_ Unsigned W64)           ), bs) else
+  if b = 0x59w then (SOME   (N_compare    (Ge_   Signed W64)           ), bs) else
+  if b = 0x5Aw then (SOME   (N_compare    (Ge_ Unsigned W64)           ), bs) else
+  if b = 0x5Bw then (SOME   (N_compare    (Eq Float W32)               ), bs) else
+  if b = 0x5Cw then (SOME   (N_compare    (Ne Float W32)               ), bs) else
+  if b = 0x5Dw then (SOME   (N_compare    (Lt W32)                     ), bs) else
+  if b = 0x5Ew then (SOME   (N_compare    (Gt W32)                     ), bs) else
+  if b = 0x5Fw then (SOME   (N_compare    (Le W32)                     ), bs) else
+  if b = 0x60w then (SOME   (N_compare    (Ge W32)                     ), bs) else
+  if b = 0x61w then (SOME   (N_compare    (Eq Float W64)               ), bs) else
+  if b = 0x62w then (SOME   (N_compare    (Ne Float W64)               ), bs) else
+  if b = 0x63w then (SOME   (N_compare    (Lt W64)                     ), bs) else
+  if b = 0x64w then (SOME   (N_compare    (Gt W64)                     ), bs) else
+  if b = 0x65w then (SOME   (N_compare    (Le W64)                     ), bs) else
+  if b = 0x66w then (SOME   (N_compare    (Ge W64)                     ), bs) else
+  if b = 0x67w then (SOME   (N_unary      (Clz    W32)                 ), bs) else
+  if b = 0x68w then (SOME   (N_unary      (Ctz    W32)                 ), bs) else
+  if b = 0x69w then (SOME   (N_unary      (Popcnt W32)                 ), bs) else
+  if b = 0x6Aw then (SOME   (N_binary     (Add Int W32)                ), bs) else
+  if b = 0x6Bw then (SOME   (N_binary     (Sub Int W32)                ), bs) else
+  if b = 0x6Cw then (SOME   (N_binary     (Mul Int W32)                ), bs) else
+  if b = 0x6Dw then (SOME   (N_binary     (Div_   Signed W32)          ), bs) else
+  if b = 0x6Ew then (SOME   (N_binary     (Div_ Unsigned W32)          ), bs) else
+  if b = 0x6Fw then (SOME   (N_binary     (Rem_   Signed W32)          ), bs) else
+  if b = 0x70w then (SOME   (N_binary     (Rem_ Unsigned W32)          ), bs) else
+  if b = 0x71w then (SOME   (N_binary     (And W32)                    ), bs) else
+  if b = 0x72w then (SOME   (N_binary     (Or W32)                     ), bs) else
+  if b = 0x73w then (SOME   (N_binary     (Xor W32)                    ), bs) else
+  if b = 0x74w then (SOME   (N_binary     (Shl W32)                    ), bs) else
+  if b = 0x75w then (SOME   (N_binary     (Shr_   Signed W32)          ), bs) else
+  if b = 0x76w then (SOME   (N_binary     (Shr_ Unsigned W32)          ), bs) else
+  if b = 0x77w then (SOME   (N_binary     (Rotl W32)                   ), bs) else
+  if b = 0x78w then (SOME   (N_binary     (Rotr W32)                   ), bs) else
+  if b = 0x79w then (SOME   (N_unary      (Clz    W64)                 ), bs) else
+  if b = 0x7Aw then (SOME   (N_unary      (Ctz    W64)                 ), bs) else
+  if b = 0x7Bw then (SOME   (N_unary      (Popcnt W64)                 ), bs) else
+  if b = 0x7Cw then (SOME   (N_binary     (Add Int W64)                ), bs) else
+  if b = 0x7Dw then (SOME   (N_binary     (Sub Int W64)                ), bs) else
+  if b = 0x7Ew then (SOME   (N_binary     (Mul Int W64)                ), bs) else
+  if b = 0x7Fw then (SOME   (N_binary     (Div_   Signed W64)          ), bs) else
+  if b = 0x80w then (SOME   (N_binary     (Div_ Unsigned W64)          ), bs) else
+  if b = 0x81w then (SOME   (N_binary     (Rem_   Signed W64)          ), bs) else
+  if b = 0x82w then (SOME   (N_binary     (Rem_ Unsigned W64)          ), bs) else
+  if b = 0x83w then (SOME   (N_binary     (And W64)                    ), bs) else
+  if b = 0x84w then (SOME   (N_binary     (Or  W64)                    ), bs) else
+  if b = 0x85w then (SOME   (N_binary     (Xor W64)                    ), bs) else
+  if b = 0x86w then (SOME   (N_binary     (Shl W64)                    ), bs) else
+  if b = 0x87w then (SOME   (N_binary     (Shr_   Signed W64)          ), bs) else
+  if b = 0x88w then (SOME   (N_binary     (Shr_ Unsigned W64)          ), bs) else
+  if b = 0x89w then (SOME   (N_binary     (Rotl W64)                   ), bs) else
+  if b = 0x8Aw then (SOME   (N_binary     (Rotr W64)                   ), bs) else
+  if b = 0x8Bw then (SOME   (N_unary      (Abs     W32)                ), bs) else
+  if b = 0x8Cw then (SOME   (N_unary      (Neg     W32)                ), bs) else
+  if b = 0x8Dw then (SOME   (N_unary      (Ceil    W32)                ), bs) else
+  if b = 0x8Ew then (SOME   (N_unary      (Floor   W32)                ), bs) else
+  if b = 0x8Fw then (SOME   (N_unary      (Trunc   W32)                ), bs) else
+  if b = 0x90w then (SOME   (N_unary      (Nearest W32)                ), bs) else
+  if b = 0x91w then (SOME   (N_unary      (Sqrt    W32)                ), bs) else
+  if b = 0x92w then (SOME   (N_binary     (Add Float W32)              ), bs) else
+  if b = 0x93w then (SOME   (N_binary     (Sub Float W32)              ), bs) else
+  if b = 0x94w then (SOME   (N_binary     (Mul Float W32)              ), bs) else
+  if b = 0x95w then (SOME   (N_binary     (Div W32)                    ), bs) else
+  if b = 0x96w then (SOME   (N_binary     (Min W32)                    ), bs) else
+  if b = 0x97w then (SOME   (N_binary     (Max W32)                    ), bs) else
+  if b = 0x98w then (SOME   (N_binary     (Copysign W32)               ), bs) else
+  if b = 0x99w then (SOME   (N_unary      (Abs     W64)                ), bs) else
+  if b = 0x9Aw then (SOME   (N_unary      (Neg     W64)                ), bs) else
+  if b = 0x9Bw then (SOME   (N_unary      (Ceil    W64)                ), bs) else
+  if b = 0x9Cw then (SOME   (N_unary      (Floor   W64)                ), bs) else
+  if b = 0x9Dw then (SOME   (N_unary      (Trunc   W64)                ), bs) else
+  if b = 0x9Ew then (SOME   (N_unary      (Nearest W64)                ), bs) else
+  if b = 0x9Fw then (SOME   (N_unary      (Sqrt    W64)                ), bs) else
+  if b = 0xA0w then (SOME   (N_binary     (Add Float W64)              ), bs) else
+  if b = 0xA1w then (SOME   (N_binary     (Sub Float W64)              ), bs) else
+  if b = 0xA2w then (SOME   (N_binary     (Mul Float W64)              ), bs) else
+  if b = 0xA3w then (SOME   (N_binary     (Div W64)                    ), bs) else
+  if b = 0xA4w then (SOME   (N_binary     (Min W64)                    ), bs) else
+  if b = 0xA5w then (SOME   (N_binary     (Max W64)                    ), bs) else
+  if b = 0xA6w then (SOME   (N_binary     (Copysign W64)               ), bs) else
+  if b = 0xA7w then (SOME   (N_convert     Wrap_i64                    ), bs) else
+  if b = 0xA8w then (SOME   (N_convert    (Trunc_f W32   Signed W32)   ), bs) else
+  if b = 0xA9w then (SOME   (N_convert    (Trunc_f W32 Unsigned W32)   ), bs) else
+  if b = 0xAAw then (SOME   (N_convert    (Trunc_f W64   Signed W32)   ), bs) else
+  if b = 0xABw then (SOME   (N_convert    (Trunc_f W64 Unsigned W32)   ), bs) else
+  if b = 0xACw then (SOME   (N_unary      (Extend_i32_   Signed)       ), bs) else
+  if b = 0xADw then (SOME   (N_unary      (Extend_i32_ Unsigned)       ), bs) else
+  if b = 0xAEw then (SOME   (N_convert    (Trunc_f W32   Signed W64)   ), bs) else
+  if b = 0xAFw then (SOME   (N_convert    (Trunc_f W32 Unsigned W64)   ), bs) else
+  if b = 0xB0w then (SOME   (N_convert    (Trunc_f W64   Signed W64)   ), bs) else
+  if b = 0xB1w then (SOME   (N_convert    (Trunc_f W64 Unsigned W64)   ), bs) else
+  if b = 0xB2w then (SOME   (N_convert    (Convert W32   Signed W32)   ), bs) else
+  if b = 0xB3w then (SOME   (N_convert    (Convert W32 Unsigned W32)   ), bs) else
+  if b = 0xB4w then (SOME   (N_convert    (Convert W64   Signed W32)   ), bs) else
+  if b = 0xB5w then (SOME   (N_convert    (Convert W64 Unsigned W32)   ), bs) else
+  if b = 0xB6w then (SOME   (N_convert     Demote                      ), bs) else
+  if b = 0xB7w then (SOME   (N_convert    (Convert W32   Signed W64)   ), bs) else
+  if b = 0xB8w then (SOME   (N_convert    (Convert W32 Unsigned W64)   ), bs) else
+  if b = 0xB9w then (SOME   (N_convert    (Convert W64   Signed W64)   ), bs) else
+  if b = 0xBAw then (SOME   (N_convert    (Convert W64 Unsigned W64)   ), bs) else
+  if b = 0xBBw then (SOME   (N_convert     Promote                     ), bs) else
+  if b = 0xBCw then (SOME   (N_convert    (Reinterpret_f W32)          ), bs) else
+  if b = 0xBDw then (SOME   (N_convert    (Reinterpret_f W64)          ), bs) else
+  if b = 0xBEw then (SOME   (N_convert    (Reinterpret_i W32)          ), bs) else
+  if b = 0xBFw then (SOME   (N_convert    (Reinterpret_i W64)          ), bs) else
+  if b = 0xC0w then (SOME   (N_unary      (Extend8_s  W32)             ), bs) else
+  if b = 0xC1w then (SOME   (N_unary      (Extend16_s W32)             ), bs) else
+  if b = 0xC2w then (SOME   (N_unary      (Extend8_s  W64)             ), bs) else
+  if b = 0xC3w then (SOME   (N_unary      (Extend16_s W64)             ), bs) else
+  if b = 0xC4w then (SOME   (N_unary       Extend32_s                  ), bs) else
+
+  (************************************)
+  (*   Variable length instructions   *)
+  (************************************)
+  (* eg, because the encoding contains a const *)
+
+  (* TODO: BOGUS until read_s and read_f properly implemented *)
+  (* Constant instructions *)
+  if b = 0x41w then   case read_s_4B bs of
+  | SOME (c32,rest) => (SOME (N_const32 Int   c32), rest)
+  | NONE            => default                                                else
+  if b = 0x42w then   case read_s_8B bs of
+  | SOME (c64,rest) => (SOME (N_const64 Int   c64), rest)
+  | NONE            => default                                                else
+  if b = 0x43w then   case read_f_4B bs of
+  | SOME (c32,rest) => (SOME (N_const32 Float c32), rest)
+  | NONE            => default                                                else
+  if b = 0x44w then case read_f_8B bs of SOME (c64,rest) => (SOME (N_const64 Float c64), rest)
+  | NONE            => default                                                else
+
+  (* trunc_sat_f. Forwhatever reason is coded as 2 bytes, instead of  *)
+  if b = 0xFCw then case read_u_4B bs of
+  | SOME (sel,rest) =>  (SOME (N_convert (Trunc_sat_f
+                          (selWidth $ sel ' 1)
+                          (selSign  $ sel ' 2)
+                          (selWidth $ sel ' 0)
+                        )) , rest)
+  | NONE            => default                                                else
+
+  default
+End
+
+
+(*
+
+
+
+  (* Curiosity (ie, not technically impt): why is the encoding not contiguous??? *)
+  if b = 0xFCw then case read_4B bs of
+    | SOME (sel, rest) => (SOME (N_convert (Trunc_sat_f
+                            (selWidth $ sel ' 1)
+                            (selSign $ sel ' 2)
+                            (selWidth $ sel ' 0)
+                          )) , rest)
+    | NONE => (NONE,b::bs)                                                    else (NONE, bs)
+  (* 0:u32 ⇒ (Trunc_sat_f W32   Signed W32)
+  1:u32 ⇒ (Trunc_sat_f W32 Unsigned W32)
+  2:u32 ⇒ (Trunc_sat_f W64   Signed W32)
+  3:u32 ⇒ (Trunc_sat_f W64 Unsigned W32)
+  4:u32 ⇒ (Trunc_sat_f W32   Signed W64)
+  5:u32 ⇒ (Trunc_sat_f W32 Unsigned W64)
+  6:u32 ⇒ (Trunc_sat_f W64   Signed W64)
+  7:u32 ⇒ (Trunc_sat_f W64 Unsigned W64) *) *)
 
 val _ = export_theory();
